coq-minuska/theories/symex.v
@@ -26,50 +26,27 @@ Equations? decouple
         (t_over (bov_variable y), singleton (y,e))
     ;
     decouple (t_term s l) avoid :=
-        let l'' := imap (fun (i : nat) (x : TermOver Expression2) =>
+        let l'' := ipfmap l (fun (i : nat) (x : TermOver Expression2) (pf : l !! i = Some x) =>
             let avoidi := avoid ∪ (union_list (vars_of <$> (take i l))) in
             let pi_sigmai := decouple x avoidi in
             pi_sigmai
-        ) l in
+        ) in
     (t_term s (fmap fst l''), union_list (fmap snd l''))
 .
 Proof.
-    Search sum_list
+    apply take_drop_middle in pf.
+    rewrite <- pf.
+    rewrite sum_list_with_compose.
+    unfold compose.
+    rewrite sum_list_with_S.
+    rewrite sum_list_fmap.
+    rewrite sum_list_with_app.
+    rewrite length_fmap.
+    rewrite length_app.
+    simpl.
+    ltac1:(lia).
 Qed.
 
-
-Fixpoint decouple
-    {Σ : StaticModel}
-    (et : TermOver Expression2)
-    (avoid : gset variable)
-    :
-    ((TermOver BuiltinOrVar)*(listset (variable * Expression2 )))%type
-:=
-match et with
-| t_over e =>
-    let y : variable := fresh (avoid) in
-    (t_over (bov_variable y), singleton (y,e))
-| t_term s l =>
-    let l'' := imap (fun (i : nat) (x : TermOver Expression2) =>
-        let avoidi := avoid ∪ (union_list (vars_of <$> (take i l))) in
-        let pi_sigmai := decouple x avoidi in
-        pi_sigmai
-    ) l in
-    (* let l'' := (fix go
-        (l' : list (TermOver Expression2))
-        (avoid' : gset variable)
-        : list ((TermOver BuiltinOrVar)*(listset (variable * Expression2 )))
-        :=
-        match l' with
-        | [] => []
-        | x::xs => 
-            let pi := decouple x (avoid' ∪ (vars_of x)) in
-            pi::(go xs (avoid' ∪ (vars_of x)))
-        end
-    ) l avoid in *)
-    (t_term s (fmap fst l''), union_list (fmap snd l''))
-end
-.
 
 Lemma decouple_avoids
     {Σ : StaticModel}
@@ -79,38 +56,34 @@ Lemma decouple_avoids
     (vars_of (decouple et avoid).1) ## avoid
 .
 Proof.
-    revert avoid.
-    induction et;
-        intros avoid;
-        simpl in *;
-        unfold vars_of;
-        simpl.
+    ltac1:(funelim (decouple et avoid)).
     {
+        ltac1:(simp decouple).
+        simpl.
+        unfold vars_of; simpl.
         unfold vars_of; simpl.
         rewrite disjoint_singleton_l.
         rewrite <- elem_of_elements.
         apply infinite_is_fresh.
     }
     {
-        revert avoid H.
-        induction l; intros avoid H; simpl in *.
-        {
-            apply disjoint_empty_l.
-        }
-        {
-            rewrite disjoint_union_l.
-            rewrite Forall_cons in H.
-            destruct H as [Hx Hxs].
-            specialize (IHl avoid Hxs).
-            clear Hxs.
-            split.
-            {
-                simpl.
-                apply Hx.
-            }
-            {
-
-            }
-        }
+        ltac1:(simp decouple).
+        simpl.
+        unfold vars_of; simpl.
+        rewrite elem_of_disjoint.
+        intros x H1x H2x.
+        rewrite elem_of_union_list in H1x.
+        destruct H1x as [X [H1X H2X]].
+        rewrite elem_of_list_fmap in H1X.
+        destruct H1X as [y [H1y H2y]].
+        rewrite elem_of_list_lookup in H2y.
+        destruct H2y as [i Hi].
+        subst.
+        rewrite list_lookup_fmap in Hi.
+        rewrite fmap_Some in Hi.
+        destruct Hi as [[t ls][HH1 HH2]].
+        simpl in *; subst.
+        apply ipfmap_lookup_Some_lt in HH1.
+        simpl in *.
     }
 Qed.
